lean/LoVe/LoVe13_BasicMathematicalStructures_ExerciseSheet.lean
@@ -17,37 +17,37 @@ namespace LoVe
 
 /- ## Question 1: Type Classes
 
-Recall the inductive type `BinTree` we introduced in lecture 5: -/
+Recall the inductive type `Tree` we introduced in lecture 5: -/
 
-#check BinTree
+#check Tree
 
 /- The following function takes two trees and attaches copies of the second
 tree to each leaf of the first tree. -/
 
-def BinTree.graft {α : Type} : BinTree α → BinTree α → BinTree α
-  | BinTree.empty,      u => u
-  | BinTree.node a l r, u =>
-    BinTree.node a (BinTree.graft l u) (BinTree.graft r u)
+def Tree.graft {α : Type} : Tree α → Tree α → Tree α
+  | Tree.nil,        u => u
+  | Tree.node a l r, u =>
+    Tree.node a (Tree.graft l u) (Tree.graft r u)
 
-#reduce BinTree.graft (BinTree.node 1 BinTree.empty BinTree.empty)
-  (BinTree.node 2 BinTree.empty BinTree.empty)
+#reduce Tree.graft (Tree.node 1 Tree.nil Tree.nil)
+  (Tree.node 2 Tree.nil Tree.nil)
 
 /- 1.1. Prove the following two theorems by structural induction on `t`. -/
 
-theorem BinTree.graft_assoc {α : Type} (t u v : BinTree α) :
-  BinTree.graft (BinTree.graft t u) v = BinTree.graft t (BinTree.graft u v) :=
+theorem Tree.graft_assoc {α : Type} (t u v : Tree α) :
+  Tree.graft (Tree.graft t u) v = Tree.graft t (Tree.graft u v) :=
   sorry
 
-theorem BinTree.graft_empty {α : Type} (t : BinTree α) :
-  BinTree.graft t BinTree.empty = t :=
+theorem Tree.graft_nil {α : Type} (t : Tree α) :
+  Tree.graft t Tree.nil = t :=
   sorry
 
-/- 1.2. Declare `BinTree` an instance of `AddMonoid` using `graft` as the
+/- 1.2. Declare `Tree` an instance of `AddMonoid` using `graft` as the
 addition operator. -/
 
 #print AddMonoid
 
-@[instance] def BinTree.AddMonoid {α : Type} : AddMonoid (BinTree α) :=
+@[instance] def Tree.AddMonoid {α : Type} : AddMonoid (Tree α) :=
   { add       :=
       sorry
     add_assoc :=
@@ -60,18 +60,18 @@ addition operator. -/
       sorry
   }
 
-/- 1.3 (**optional**). Explain why `BinTree` with `graft` as addition cannot
-be declared an instance of `AddGroup`. -/
+/- 1.3 (**optional**). Explain why `Tree` with `graft` as addition cannot be
+declared an instance of `AddGroup`. -/
 
 #print AddGroup
 
 -- enter your explanation here
 
-/- 1.4 (**optional**). Prove the following theorem illustrating why `BinTree`
+/- 1.4 (**optional**). Prove the following theorem illustrating why `Tree`
 with `graft` as addition does not constitute an `AddGroup`. -/
 
-theorem BinTree.add_left_neg_counterexample :
-  ∃x : BinTree ℕ, ∀y : BinTree ℕ, BinTree.graft y x ≠ BinTree.empty :=
+theorem Tree.add_left_neg_counterexample :
+  ∃x : Tree ℕ, ∀y : Tree ℕ, Tree.graft y x ≠ Tree.nil :=
   sorry
 
 
@@ -85,7 +85,7 @@ Recall the following definitions from the lecture: -/
 /- 2.1. Prove that the finite set of nodes does not change when mirroring a
 tree. -/
 
-theorem Finset.elems_mirror (t : BinTree ℕ) :
+theorem Finset.elems_mirror (t : Tree ℕ) :
   Finset.elems (mirror t) = Finset.elems t :=
   sorry
 
@@ -94,14 +94,14 @@ tree `t` for which `List.elems t ≠ List.elems (mirror t)`.
 
 If you define a suitable counterexample, the proof below will succeed. -/
 
-def rottenTree : BinTree ℕ :=
+def rottenTree : Tree ℕ :=
   sorry
 
 #eval List.elems rottenTree
 #eval List.elems (mirror rottenTree)
 
 theorem List.elems_mirror_counterexample :
-  ∃t : BinTree ℕ, List.elems t ≠ List.elems (mirror t) :=
+  ∃t : Tree ℕ, List.elems t ≠ List.elems (mirror t) :=
   by
     apply Exists.intro rottenTree
     simp [List.elems]
